proof/correctness/avx2/MLKEM_keccak_avx2.ec
@@ -1,0 +1,355 @@
+require import AllCore IntDiv List.
+from Jasmin require import JModel.
+
+
+require Jkem_avx2.
+
+require import Keccak1600_Spec.
+
+import FIPS202_SHA3_Spec.
+import Keccakf1600_Spec.
+
+require import Array7.
+
+
+(* MLKEM array sizes *)
+require import Array536. (* BUF_SIZE *)
+require import Array32.  (* SEED SIZE *)
+require import Array4.   (* mat. indexes *)
+
+op stmatch_avx2 (st: FIPS202_Keccakf1600.state) (stavx2: W256.t Array7.t): bool.
+
+op stavx2bytes (stavx2: W256.t Array7.t): W8.t list.
+
+
+
+hoare stavx2_unpack_at_h _st _buf _at:
+ Jkem_avx2.M(Jkem_avx2.Syscall)._stavx2_unpack_at
+ : state = _st
+   /\ buf = _buf
+   /\ offset = _at
+   ==>
+   sub _buf 0 (to_uint _at) = sub res 0 (to_uint _at)
+   /\ sub res (to_uint _at) 200 = stavx2bytes _st.
+(*
+   buf_subl res 0 (to_uint _at+200)
+   = buf_subl _buf 0 (to_uint _at) ++ stavx2bytes _st.
+proc.
+*)
+admitted.
+
+lemma stavx2_unpack_at_ll:
+ islossless Jkem_avx2.M(Jkem_avx2.Syscall)._stavx2_unpack_at.
+proof. by islossless. qed.
+
+phoare stavx2_unpack_at_ph _st _buf _at:
+ [ Jkem_avx2.M(Jkem_avx2.Syscall)._stavx2_unpack_at
+   : state = _st
+     /\ buf = _buf
+     /\ offset = _at
+     ==>
+   sub _buf 0 (to_uint _at) = sub res 0 (to_uint _at)
+   /\ sub res (to_uint _at) 200 = stavx2bytes _st
+(*
+     buf_subl res 0 (to_uint _at+200)
+     = buf_subl _buf 0 (to_uint _at) ++ stavx2bytes _st
+*)
+ ] = 1%r.
+proof.
+by conseq stavx2_unpack_at_ll (stavx2_unpack_at_h _st _buf _at).
+qed.
+
+phoare stavx2_pack_at_ph _buf _at:
+ [ Jkem_avx2.M(Jkem_avx2.Syscall)._stavx2_pack_at
+   : st = _buf
+     /\ offset = _at
+     ==>
+     stavx2bytes res = sub _buf (to_uint _at) 200
+ ] = 1%r.
+proof.
+admitted.
+
+hoare xof_init_avx2_h _rho _rc:
+ Jkem_avx2.M(Jkem_avx2.Syscall).xof_init_avx2
+ : rho = _rho /\ index = _rc
+   ==>
+   stmatch_avx2 (SHAKE128_ABSORB (to_list _rho ++ W2u8.to_list _rc)) res.
+proof.
+proc; simplify.
+admitted.
+
+lemma xof_init_avx2_ll:
+ islossless Jkem_avx2.M(Jkem_avx2.Syscall).xof_init_avx2.
+proof.
+islossless.
+while (true) (7-i).
+ by move=> z; auto => /> /#.
+by auto => /> /#.
+qed.
+
+phoare xof_init_avx2_ph _rho _rc:
+ [ Jkem_avx2.M(Jkem_avx2.Syscall).xof_init_avx2
+   : rho = _rho /\ index = _rc
+     ==>
+     stmatch_avx2 (SHAKE128_ABSORB (to_list _rho ++ W2u8.to_list _rc)) res
+ ] = 1%r.
+proof. by conseq xof_init_avx2_ll (xof_init_avx2_h _rho _rc). qed.
+
+
+
+op state_stavx2_match (st: W64.t Array25.t) (stavx2: W256.t Array7.t): bool.
+
+op st25_to_stavx2 (st: W64.t Array25.t): W256.t Array7.t.
+op stavx2_to_st25 (stavx2: W256.t Array7.t): W64.t Array25.t.
+
+
+hoare keccakf1600_avx2_h (_st: W64.t Array25.t):
+ Jkem_avx2.M(Jkem_avx2.Syscall)._keccakf1600_avx2
+ : stmatch_avx2 _st state
+ ==> stmatch_avx2 (Keccakf1600_Spec.keccak_f1600_op _st) res.
+admitted.
+
+lemma keccakf1600_avx2_ll: islossless Jkem_avx2.M(Jkem_avx2.Syscall)._keccakf1600_avx2.
+proof.
+admitted.
+
+phoare keccakf1600_avx2_ph (_st: W64.t Array25.t):
+ [ Jkem_avx2.M(Jkem_avx2.Syscall)._keccakf1600_avx2
+ : stmatch_avx2 _st state
+ ==> stmatch_avx2 (Keccakf1600_Spec.keccak_f1600_op _st) res ] = 1%r.
+proof. by conseq keccakf1600_avx2_ll (keccakf1600_avx2_h _st). qed.
+
+type state4x = W256.t Array25.t.
+type state = W64.t Array25.t.
+op (\a25bits64) (a: state4x) (k: int): state =
+ Array25.map (fun (x: W256.t) => W4u64.\bits64 x k) a.
+
+op a25pack4 (l: state list): state4x =
+ Array25.init (fun i => pack4 (map (fun (s: state) => s.[i]) l)).
+
+op a25unpack4 (st4: state4x): state list =
+ map (fun k=> st4 \a25bits64 k) (iota_ 0 4).
+
+lemma a25bits64iE x k i:
+ 0 <= i < 25 =>
+ (x \a25bits64 k).[i] = x.[i] \bits64 k.
+proof. by move=> Hi; rewrite mapiE //. qed.
+
+lemma a25unpack4K s4:
+ a25pack4 (a25unpack4 s4) = s4.
+proof.
+rewrite /a25pack4 /a25unpack4.
+apply Array25.ext_eq => i Hi; rewrite initiE //=.
+rewrite -iotaredE /= !a25bits64iE //=.
+rewrite -{5}(unpack64K s4.[i]); congr.
+by rewrite unpack64E init_of_list -iotaredE /=. 
+qed.
+
+op st0: state = Array25.create W64.zero.
+
+lemma a25pack4_bits64 k (stl: state list):
+ 0 <= k < 4 =>
+ a25pack4 stl \a25bits64 k = nth st0 stl k.
+proof.
+move=> Hk; apply Array25.ext_eq => i Hi.
+rewrite mapiE //= initiE //= pack4bE //=.
+rewrite of_listE initiE //=.
+case: (k < size stl) => E.
+ by rewrite (nth_map st0) 1:/#.
+rewrite !nth_out; first 2 by smt(size_map).
+by rewrite createiE.
+qed.
+
+op match_state4x (st0 st1 st2 st3: state) (st4x: state4x) =
+ st4x = a25pack4 [st0; st1; st2; st3].
+
+lemma a25pack4_eq stl st4x:
+ a25pack4 stl = st4x
+ <=>
+ all (fun k=>st4x \a25bits64 k = nth st0 stl k) (iota_ 0 4).
+proof.
+split.
+ move => <-; apply/List.allP => k. 
+ rewrite mem_iota => Hk /=; apply a25pack4_bits64; smt().
+move=> /List.allP H.
+apply Array25.ext_eq => i Hi.
+rewrite initiE //=.
+rewrite -(unpack64K st4x.[i]); congr.
+apply W4u64.Pack.ext_eq => k Hk.
+rewrite of_listE unpack64E !initiE //=.
+rewrite -a25bits64iE // H; first smt(mem_iota).
+case: (k < size stl) => E.
+ by rewrite (nth_map st0) 1:/#.
+rewrite !nth_out; first 2 by smt(size_map).
+by rewrite createiE.
+qed.
+
+lemma xorw_bits64 (w1 w2: W256.t) k:
+ 0 <= k < 4 =>
+ w1 `^` w2 \bits64 k = (w1 \bits64 k) `^` (w2 \bits64 k).
+proof.
+move=> Hk; rewrite -{1}(unpack64K w1) -{1}(unpack64K w2). 
+by rewrite xorb4u64E pack4bE // map2iE // !unpack64E !initiE.
+qed.
+
+lemma invw_bits64 (w: W256.t) k:
+ 0 <= k < 4 =>
+ invw w \bits64 k = invw (w \bits64 k).
+proof. by move=> Hk; rewrite -{1}(unpack64K w) invw64E //. qed.
+
+op map_state4x (f:state->state) (st:state4x): state4x =
+ a25pack4 (map f (a25unpack4 st)).
+
+lemma map_state4x_neq r a:
+ r <> map_state4x keccak_f1600_op a
+ <=> (r \a25bits64 0) <> keccak_f1600_op (a \a25bits64 0) \/
+     (r \a25bits64 1) <> keccak_f1600_op (a \a25bits64 1) \/
+     (r \a25bits64 2) <> keccak_f1600_op (a \a25bits64 2) \/
+     (r \a25bits64 3) <> keccak_f1600_op (a \a25bits64 3).
+proof.
+rewrite /map_state4x eq_sym a25pack4_eq -iotaredE /=.
+rewrite !(nth_map st0); first 4 by rewrite /a25unpack4 size_map size_iota.
+by rewrite /a25unpack4 -iotaredE /= /#.
+qed.
+
+hoare keccakf1600_4x_h (_a: state4x):
+ Jkem_avx2.M(Jkem_avx2.Syscall)._keccakf1600_4x :
+ a = _a
+ ==> res = map_state4x keccak_f1600_op _a.
+proof.
+admitted.
+
+lemma keccakf1600_4x_round_ll:
+ islossless Jkem_avx2.M(Jkem_avx2.Syscall).keccakf1600_4x_round.
+admitted.
+
+lemma keccakf1600_4x_ll:
+ islossless Jkem_avx2.M(Jkem_avx2.Syscall)._keccakf1600_4x.
+proof.
+islossless.
+while (true) (768 - to_uint c).
+ move=> z.
+ wp; call keccakf1600_4x_round_ll.
+ wp; call keccakf1600_4x_round_ll.
+ auto => /> &m.
+ by rewrite ultE to_uintD of_uintK /#.
+by auto => /> c; rewrite ultE of_uintK /#.
+qed.
+
+phoare keccakf1600_4x_ph (_a: state4x):
+ [ Jkem_avx2.M(Jkem_avx2.Syscall)._keccakf1600_4x :
+   a = _a
+   ==> res = map_state4x keccak_f1600_op _a ] = 1%r.
+proof. by conseq keccakf1600_4x_ll (keccakf1600_4x_h _a). qed.
+
+lemma st_i_add st a b:
+ 0 <= a => 0 <= b =>
+ st_i (FIPS202_SHA3_Spec.st_i st b) a
+ = st_i st (a+b).
+proof.
+rewrite /st_i.
+elim/natind: a b.
+ move=> n Hn b Ha Hb; rewrite (iter0 n) /#.
+move=> n Hn IH b Ha Hb.
+by rewrite eq_sym (:n+1+b=n+b+1) 1:/# (iterS (n+b)) 1:/# -IH // iterS 1:/#.
+qed.
+
+hoare xof_init_x4_h _rho _idxs:
+ Jkem_avx2.M(Jkem_avx2.Syscall).xof_init_x4
+ : rho = _rho /\ indexes = _idxs
+   ==>
+   match_state4x
+    (SHAKE128_ABSORB (to_list _rho ++ W2u8.to_list _idxs.[0])) 
+    (SHAKE128_ABSORB (to_list _rho ++ W2u8.to_list _idxs.[1])) 
+    (SHAKE128_ABSORB (to_list _rho ++ W2u8.to_list _idxs.[2])) 
+    (SHAKE128_ABSORB (to_list _rho ++ W2u8.to_list _idxs.[3])) 
+    res.
+proof.
+proc; simplify.
+admit.
+qed.
+
+lemma xof_init_x4_ll: islossless Jkem_avx2.M(Jkem_avx2.Syscall).xof_init_x4.
+proof.
+islossless.
++ while (true) (25-i).
+   by move=> z; auto => /> /#.
+  by auto => /> /#.
++ while (true) (4-i).
+   by move=> z; auto => /> /#.
+  by auto => /> /#.
+while (true) (4-i).
+ by move=> z; auto => /> /#.
+by auto => /> /#.
+qed.
+
+phoare xof_init_x4_ph _rho _idxs:
+ [ Jkem_avx2.M(Jkem_avx2.Syscall).xof_init_x4
+   : rho = _rho /\ indexes = _idxs
+     ==>
+     match_state4x
+      (SHAKE128_ABSORB (to_list _rho ++ W2u8.to_list _idxs.[0])) 
+      (SHAKE128_ABSORB (to_list _rho ++ W2u8.to_list _idxs.[1])) 
+      (SHAKE128_ABSORB (to_list _rho ++ W2u8.to_list _idxs.[2])) 
+      (SHAKE128_ABSORB (to_list _rho ++ W2u8.to_list _idxs.[3])) 
+      res ] = 1%r.
+proof. by conseq xof_init_x4_ll (xof_init_x4_h _rho _idxs). qed.
+
+hoare st4x_unpack_at_h _st0 _st1 _st2 _st3 _buf0 _buf1 _buf2 _buf3 _at:
+ Jkem_avx2.M(Jkem_avx2.Syscall).__st4x_unpack_at
+ : match_state4x _st0 _st1 _st2 _st3 st4x
+   /\ buf0=_buf0 /\ buf1=_buf1 /\ buf2=_buf2 /\ buf3=_buf3
+   /\ offset=_at
+   ==> sub _buf0 0 (to_uint _at) = sub res.`1 0 (to_uint _at)
+       /\ sub _buf1 0 (to_uint _at) = sub res.`2 0 (to_uint _at)
+       /\ sub _buf2 0 (to_uint _at) = sub res.`3 0 (to_uint _at)
+       /\ sub _buf3 0 (to_uint _at) = sub res.`4 0 (to_uint _at)
+       /\ sub res.`1 (to_uint _at) 200 = state2bytes _st0
+       /\ sub res.`2 (to_uint _at) 200 = state2bytes _st1
+       /\ sub res.`3 (to_uint _at) 200 = state2bytes _st2
+       /\ sub res.`4 (to_uint _at) 200 = state2bytes _st3.
+proof.
+proc.
+admitted.
+
+lemma stmatch_avx2_bytes st stavx:
+ stmatch_avx2 st stavx <=>
+ state2bytes st = stavx2bytes stavx.
+proof.
+admitted.
+
+(*
+lemma stavx2_bytes_squeeze at (buf: W8.t Array536.t) st stavx:
+ stmatch_avx2 st stavx =>
+ sub buf at 200 = stavx2bytes stavx =>
+ sub buf at 168 = squeezestate st 168.
+proof.
+move => /stmatch_avx2_bytes Hm.
+rewrite -Hm /squeezestate => <-.
+by rewrite /sub take_mkseq /#.
+qed.
+*)
+
+phoare st4x_unpack_at_ph _st0 _st1 _st2 _st3 _buf0 _buf1 _buf2 _buf3 _at:
+ [ Jkem_avx2.M(Jkem_avx2.Syscall).__st4x_unpack_at
+   : match_state4x _st0 _st1 _st2 _st3 st4x
+     /\ buf0=_buf0 /\ buf1=_buf1 /\ buf2=_buf2 /\ buf3=_buf3
+     /\ offset=_at
+     ==> sub _buf0 0 (to_uint _at) = sub res.`1 0 (to_uint _at)
+         /\ sub _buf1 0 (to_uint _at) = sub res.`2 0 (to_uint _at)
+         /\ sub _buf2 0 (to_uint _at) = sub res.`3 0 (to_uint _at)
+         /\ sub _buf3 0 (to_uint _at) = sub res.`4 0 (to_uint _at)
+         /\ sub res.`1 (to_uint _at) 200 = state2bytes _st0
+         /\ sub res.`2 (to_uint _at) 200 = state2bytes _st1
+         /\ sub res.`3 (to_uint _at) 200 = state2bytes _st2
+         /\ sub res.`4 (to_uint _at) 200 = state2bytes _st3 ] = 1%r.
+proof.
+proc.
+admitted.
+
+lemma stx4_map_keccakf st0 st1 st2 st3 stx4:
+ match_state4x st0 st1 st2 st3 stx4 =>
+ match_state4x (keccak_f1600_op st0) (keccak_f1600_op st1) (keccak_f1600_op st2) (
+  keccak_f1600_op st3) (map_state4x keccak_f1600_op stx4).
+admitted.
+
